lakefile.lean
@@ -1,12 +1,10 @@
 import Lake
 open Lake DSL
 
-package foo {
-  -- add package configuration options here
-}
+package formal_systems
 
-require mathlib 
-  from git "https://github.com/leanprover-community/mathlib4"
+require mathlib
+  from git "https://github.com/leanprover-community/mathlib4"@"v4.2.0"
 
 @[default_target]
 lean_lib FormalSystems
